Skip.thy: added simp rules, removed unnecessary 'unskip' constant.

isa/Skip.thy
@@ -2,19 +2,22 @@ theory Skip
 imports Main
 begin
 
-subsection {* skip and unskip *}
+subsection {* skip *}
+
+text {* The function @{text "skip i"} enumerates all naturals except
+@{text "i"}. *}
 
 definition
   skip :: "nat \<Rightarrow> nat \<Rightarrow> nat" where
-  "skip i n = (if n < i then n else Suc n)"
+  "skip i = (\<lambda>n. if n < i then n else Suc n)"
 
-lemma skip_0: "skip 0 n = Suc n"
+lemma skip_0 [simp]: "skip 0 = Suc"
 unfolding skip_def by simp
 
-lemma skip_Suc_Suc: "skip (Suc i) (Suc n) = Suc (skip i n)"
+lemma skip_Suc_Suc [simp]: "skip (Suc i) (Suc n) = Suc (skip i n)"
 unfolding skip_def by simp
 
-lemma skip_Suc_0: "skip (Suc i) 0 = 0"
+lemma skip_Suc_0 [simp]: "skip (Suc i) 0 = 0"
 unfolding skip_def by simp
 
 lemma skip_inject: "(skip i m = skip i n) = (m = n)"
@@ -31,98 +34,38 @@ unfolding skip_def by auto
 lemma skip_neq: "skip i n \<noteq> i"
 unfolding skip_def by simp
 
-definition
-  unskip :: "nat \<Rightarrow> nat \<Rightarrow> nat" where
-  "unskip i n = (if i < n then (n - 1) else n)"
-
-lemma unskip_i_0: "unskip i 0 = 0"
-unfolding unskip_def by simp
-
-lemma unskip_0_Suc: "unskip 0 (Suc n) = n"
-unfolding unskip_def by simp
-
-lemma unskip_Suc_Suc: "unskip (Suc i) (Suc n) = Suc (unskip i n)"
-unfolding unskip_def by simp
-
-lemma unskip_skip: "unskip i (skip i n) = n"
-unfolding unskip_def skip_def by simp
-
-lemma skip_unskip: "n \<noteq> i \<Longrightarrow> skip i (unskip i n) = n"
-unfolding skip_def unskip_def by auto
-
 lemma skip_cases:
   assumes 1: "x = i \<Longrightarrow> P"
   assumes 2: "\<And>n. x = skip i n \<Longrightarrow> P"
   shows "P"
-apply (case_tac "x = i")
-apply (erule 1)
-apply (erule 2 [OF skip_unskip [symmetric]])
-done
-
-lemma unskip_inject: "\<lbrakk>m \<noteq> i; n \<noteq> i\<rbrakk> \<Longrightarrow> (unskip i m = unskip i n) = (m = n)"
-apply safe
-apply (drule skip_inject [where i="i", THEN iffD2])
-apply (simp add: skip_unskip)
+apply (cases "x = i", erule 1)
+apply (rule 2 [where n="if i < x then (x - 1) else x"])
+apply (auto simp add: skip_def)
 done
 
 subsection {* substVar *}
 
-definition
-  substVar :: "(nat \<Rightarrow> 'a) \<Rightarrow> nat \<Rightarrow> 'a \<Rightarrow> nat \<Rightarrow> 'a" where
-  "substVar V i x n = (if n = i then x else V (unskip i n))"
+definition substVar :: "(nat \<Rightarrow> 'a) \<Rightarrow> nat \<Rightarrow> 'a \<Rightarrow> nat \<Rightarrow> 'a"
+  where "substVar V i x n =
+    (if n = i then x else V (if i < n then (n - 1) else n))"
 
-lemma substVar_eq: "substVar V i x i = x"
+lemma substVar_0_0: "substVar V 0 x 0 = x"
 unfolding substVar_def by simp
 
-lemma substVar_neq: "n \<noteq> i \<Longrightarrow> substVar V i x n = V (unskip i n)"
+lemma substVar_0_Suc [simp]: "substVar V 0 x (Suc n) = V n"
 unfolding substVar_def by simp
 
-lemma substVar_lt: "n < i \<Longrightarrow> substVar V i x n = V n"
-unfolding substVar_def unskip_def by simp
-
-lemma substVar_gt: "i < n \<Longrightarrow> substVar V i x n = V (n - 1)"
-unfolding substVar_def unskip_def by simp
-
-lemma substVar_Var:
-  "substVar V i (V m) n = V (if n = i then m else unskip i n)"
+lemma substVar_Suc_0 [simp]: "substVar V (Suc i) x 0 = V 0"
 unfolding substVar_def by simp
 
-lemma substVar_skip: "substVar V i x (skip i n) = V n"
-unfolding substVar_def by (simp add: skip_neq unskip_skip)
+lemma substVar_Suc_Suc [simp]:
+  "substVar V (Suc i) x (Suc n) = substVar (\<lambda>n. V (Suc n)) i x n"
+unfolding substVar_def by simp
 
-lemma lift_substVar_le:
-  assumes lift_V: "\<And>n. lift i (V n) = V (skip i n)"
-  shows "i \<le> j \<Longrightarrow>
-       lift i (substVar V j x n) =
-       substVar V (Suc j) (lift i x) (skip i n)"
-apply (rule_tac x="n" and i="j" in skip_cases)
-apply (simp add: skip_def substVar_eq)
-apply (simp add: substVar_skip skip_skip_le lift_V)
-done
+lemma substVar_eq [simp]: "substVar V i x i = x"
+unfolding substVar_def by simp
 
-lemma lift_substVar_ge:
-  assumes lift_V: "\<And>n. lift i (V n) = V (skip i n)"
-  shows "j \<le> i \<Longrightarrow>
-       lift i (substVar V j x n) =
-       substVar V j (lift i x) (skip (Suc i) n)"
-apply (rule_tac x="n" and i="j" in skip_cases)
-apply (simp add: skip_def substVar_eq)
-apply (simp add: substVar_skip skip_Suc_skip lift_V)
-done
-
-lemma subst_substVar_ge:
-  assumes subst_lift: "\<And>x. subst j (lift j y) x = y"
-  assumes lift_V: "\<And>i n. lift i (V n) = V (skip i n)"
-  assumes subst_V: "\<And>i n x. subst i (V n) x = substVar V i x n"
-  shows "j \<le> i \<Longrightarrow>
-       subst i (substVar V j x n) y =
-       subst j (substVar V (Suc i) (lift j y) n) (subst i x y)"
- apply (rule_tac x="n" and i="j" in skip_cases)
-  apply (rule_tac x="n" and i="Suc i" in skip_cases)
-   apply simp
-  apply (clarsimp simp add: subst_V substVar_eq substVar_skip)
-  apply (clarsimp simp add: skip_def substVar_eq)
- apply (clarsimp simp add: subst_V substVar_skip)
-by (auto simp add: assms substVar_def unskip_def skip_def)
+lemma substVar_skip [simp]: "substVar V i x (skip i n) = V n"
+unfolding substVar_def skip_def by auto
 
 end
